
Let's look at an example:
$$f(x) = \frac{1}{1-x}$$
We know
$$\begin{align} 
&(-ln(1-x))'  \\
&= \frac{d}{dx} (-ln(1-x))=\frac{1}{1-x} \\
 &\implies d(-ln(1-x)) = \frac{1}{1-x}dx
  \end{align}$$

# Example

Find solutions for $$\frac{dF}{dx}= \frac{1}{1-x}$$over $(- \infty, 1)$ 


By the above, $$F(x) = -ln(1-x) + C$$ solves the equation

<i> Question: can we find any other Solution? </i>
If F solves the equation, then
$$\begin{align}
\frac{dF}{dx} &= \frac{1}{1-x} \\
\frac{d}{dx}(-ln(1-x)) &= \frac{1}{1-x} \\
&\implies \frac{d}{dx}(F-(-ln(1-x)))=0 \\
&F = -ln(1-x)+C

\end{align}$$


Graphs of the solutions:
![[Pasted image 20240108120628.png]]
(The green graphs give solutions for $$\frac{d}{dx}(-ln(1-x))=\frac{1}{1-x}$$ over x>0
)


## Indefinite integral
We usually denote $$\int \frac{1}{1-x}dx = -ln(1-x) +C$$ called the indefinite integral of 1/1-x

Essentially finding the indefinite integrals are inverse of taking derivatives


